theories/TM/Code/ProgrammingTools.v
@@ -7,45 +7,6 @@ Require Import Lia.
 (** All Coq modules in that the user programms Turing machine should [From Undecidability Require Import TM.Code.ProgrammingTools]. The module should additionally require and import the modules containing the constructor and deconstructor machines, e.g. [Require Import TM.Code.CaseNat], etc. *)
 
 
-
-
-(** This tactic automatically solves/instantiates premises of a hypothesis. If the hypothesis is a conjunction, it is destructed. *)
-Ltac modpon' H :=
-  simpl_surject;
-  once lazymatch type of H with
-  | forall (i : Fin.t _), ?P => idtac
-  | forall (x : ?X), ?P =>
-    once lazymatch type of X with
-    | Prop =>
-      tryif spec_assert H by
-          (simpl_surject;
-           solve [ eauto
-                 | contains_ext
-                 | isVoid_mono
-                 ]
-          )
-      then idtac (* "solved premise of type" X *);
-           modpon' H
-      else (spec_assert H;
-            [ idtac (* "could not solve premise" X *) (* new goal for the user *)
-            | modpon' H (* continue after the user has proved the premise manually *)
-            ]
-           )
-    | _ =>
-      (* instantiate variable [x] with evar *)
-      let x' := fresh "x" in
-      evar (x' : X); specialize (H x'); subst x';
-      modpon' H
-    end
-  | ?X /\ ?Y =>
-    let H' := fresh H in
-    destruct H as [H H']; modpon' H; modpon' H'
-  | _ => idtac
-  end.
-
-Ltac modpon H := progress (modpon' H).
-
-
 (** To get rid of all those uggly tape rewriting hypothesises. Be warned that maybe the goal can't be solved after that. *)
 Ltac clear_tape_eqs :=
   repeat once lazymatch goal with
