theories/TM/Compound/TMTac.v
@@ -1,7 +1,44 @@
 From Undecidability Require Import TM.Util.Prelim TM.Util.TM_facts.
-From Undecidability Require Import TM.Lifting.LiftTapes. (* for [simpl_not_in] *)
+From Undecidability.TM Require Import Lifting.LiftTapes CodeTM ChangeAlphabet. (* for [simpl_not_in] *)
 
 (** * Tactics that help verifying complex machines *)
+
+
+(** This tactic automatically solves/instantiates premises of a hypothesis. If the hypothesis is a conjunction, it is destructed. *)
+Ltac modpon' H :=
+  simpl_surject;
+  once lazymatch type of H with
+  | forall (i : Fin.t _), ?P => idtac
+  | forall (x : ?X), ?P =>
+    once lazymatch type of X with
+    | Prop =>
+      tryif spec_assert H by
+          (simpl_surject;
+           solve [ eauto
+                 | contains_ext
+                 | isVoid_mono
+                 ]
+          )
+      then idtac (* "solved premise of type" X *);
+           modpon' H
+      else (spec_assert H;
+            [ idtac (* "could not solve premise" X *) (* new goal for the user *)
+            | modpon' H (* continue after the user has proved the premise manually *)
+            ]
+           )
+    | _ =>
+      (* instantiate variable [x] with evar *)
+      let x' := fresh "x" in
+      evar (x' : X); specialize (H x'); subst x';
+      modpon' H
+    end
+  | ?X /\ ?Y =>
+    let H' := fresh H in
+    destruct H as [H H']; modpon' H; modpon' H'
+  | _ => idtac
+  end.
+
+Ltac modpon H := progress (modpon' H).
 
 
 Ltac dec_pos P := let H := fresh in destruct (Dec P) as [_ | H]; [ | now contradiction H].
